%
% Welcome to Overleaf --- just edit your LaTeX on the left,
% and we'll compile it for you on the right. If you open the
% 'Share' menu, you can invite other users to edit at the same
% time. See www.overleaf.com/learn for more info. Enjoy!
%
%%%%%%%%%%%%%%%%%%%%%%%%%%%%%%%%%%%%%%%%%%%%%%%%%%%%%%%%%%%%%%%


% Inbuilt themes in beamer
\documentclass{beamer}

% Theme choice:
\usetheme{CambridgeUS}

% Title page details: 
\title{Papoulis Question 6.60} 
\author{Suryaansh Jain}
\date{\today}
\logo{\large \LaTeX{}}

\providecommand{\pr}[1]{\ensuremath{\Pr\left(#1\right)}}


\begin{document}

% Title page frame
\begin{frame}
    \titlepage 
\end{frame}

% Remove logo from the next slides
\logo{}


% Outline frame
\begin{frame}{Outline}
    \tableofcontents
\end{frame}


\section{Question}
\begin{frame}{Question}

$x$ and $y$ are independent exponential random variables with common parameter $\lambda$. Find \\
(a) $E[\text{min}(x, y)]$ \\
(b) $E[\text{max}(2x, y)]$.
\end{frame}

\section{Solution}
\begin{frame}{Genaral}
    \begin{equation}
        f(x) = 
        \begin{cases}
            \lambda e^{-\lambda x}, & x \geq 0 \\
            0, & otherwise
        \end{cases}
    \end{equation}
        
    \begin{equation}
        f(y) = 
        \begin{cases}
            \lambda e^{-\lambda y}, & y \geq 0 \\
            0, & otherwise
        \end{cases}
    \end{equation}
\end{frame} 

\begin{frame}{Part (a)}

    Let $w = \text{min}(x,y)$
    Then from inclusion-exclusion,
    \begin{equation}
        F_w(w) = F_x(w) + F_y(w) - F_x(w).F_y(w)
    \end{equation}
    Differentiating,
    \begin{equation}
        f_w(w) = f_x(w) + f_y(w) - f_x(w).F_y(w) - F_x(w).f_y(w)
    \end{equation}
    
    Plugging the values of $f_x(w)$ and $f_y(w)$,
    
    \begin{equation}
        f_w(w) = 2\lambda e^{-2\lambda w}
    \end{equation}
    
    As this an exponential variable its expected value is,
    
    \begin{equation}
        E(\text{min}(x,y)) = \frac{1}{2\lambda}
    \end{equation}
    
\end{frame} 

\begin{frame}{Part (b)}
    Let $z = \text{man}(2x,y)$
    Then,
    \begin{align}
        F_w(w) &= P(\text{max}(2x, y) \leq z) \\
        &= P(2x \leq z, 2x \geq y) + P(y \leq z, y \geq 2x) \\
        &= P(2x \leq z, y \leq z) \\
        &= F_{xy}(z/2 , z)
    \end{align}
    
    As $x$ ans $y$ are independent $F_{xy}(z/2 , z) = F_x(z/2).F_y(z)$
    \begin{equation}
        F_w(w) = F_x(z/2).F_y(z)
    \end{equation}
\end{frame}

\begin{frame}{Part (b) Contd.}
    Differentiating, 
    \begin{align}
        f_z(z) &= F_x(z/2).f_y(z) + \frac{1}{2} f_x(z/2).F_y(z)\\
        &= \left(1 - e^{-\lambda z/2} \right).e^{-\lambda z} + \frac{1}{2}\left(1 - e^{\lambda z} \right).e^{-\lambda z/2}\\
        &= \lambda e^{-\lambda z} - \frac{3}{2}\lambda e^{-\frac{3}{2}\lambda z} + \frac{1}{2}\lambda e^{-\frac{1}{2}\lambda z} \\
        &\implies E(z) = \frac{1}{\lambda} - \frac{2}{3\lambda} + \frac{2}{\lambda} = \frac{7}{3\lambda}
    \end{align}
\end{frame}

\end{document}

